Wip

Semantic/Stlc/RebindTheory.lean
@@ -1,31 +1,54 @@
 import Semantic.Stlc.TypeSystem
 import Semantic.Stlc.Interpreter
+import Semantic.Stlc.Denotation
 import Mathlib.Tactic
-
-def hello : Nat := 42
 
 structure Rebind (s1 : Store n1) (f : Rename n1 n2) (s2 : Store n2) where
   var : ∀ (x : Var n1),
     s2.lookup (f.var x) = (s1.lookup x).rename f
 
+def Rebind.liftVar (ρ : Rebind s1 f s2) :
+  Rebind (s1.val v0) (f.liftVar) (s2.val (v0.rename f)) where
+  var := fun
+  | .here => by
+    conv => lhs; simp [Rename.liftVar]
+    simp [Store.lookup]
+    simp [Exp.rename_succVar_comm]
+  | .there x => by
+    have h := ρ.var x
+    conv => lhs; simp [Rename.liftVar]
+    simp [Store.lookup]
+    simp [<-Exp.rename_succVar_comm]
+    congr
+
 def Eval.rebind {f : Rename n1 n2}
   (hev : Eval s1 e1 v1)
   (ρ : Rebind s1 f s2) :
   Eval s2 (e1.rename f) (v1.rename f) := by
-  induction hev generalizing n2
+  induction hev generalizing n2 <;> try (solve | grind [Eval, Exp.rename])
   case ev_var x0 =>
     have h := ρ.var x0
     simp [<-h]
     grind [Exp.rename, Eval]
-  case ev_app ih1 ih2 => sorry
-  case ev_abs => sorry
-  case ev_nsucc ih => sorry
-  case ev_btrue => sorry
-  case ev_bfalse => sorry
-  case ev_nzero => sorry
-  case ev_pred_nzero ih => sorry
-  case ev_pred_nsucc ih => sorry
-  case ev_iszero_nzero ih => sorry
-  case ev_iszero_nsucc ih => sorry
-  case ev_cond_true ih1 ih2 => sorry
-  case ev_cond_false ih1 ih2 => sorry
+  case ev_app ih1 ih2 ih3 =>
+    simp [Exp.openVar_rename_comm]
+    apply ev_app
+    { apply ih1 ρ }
+    { apply ih2 ρ }
+    { apply ih3
+      apply ρ.liftVar }
+  case ev_nsucc ih =>
+    apply ev_nsucc
+    · apply ih; apply ρ
+    · grind [Exp.rename_is_numval]
+  case ev_pred_nsucc ih =>
+    apply ev_pred_nsucc
+    · apply ih; apply ρ
+    · grind [Exp.rename_is_numval]
+  case ev_iszero_nsucc ih =>
+    apply ev_iszero_nsucc
+    · apply ih; apply ρ
+    · grind [Exp.rename_is_numval]
+
+def Rebind.succVar : Rebind s1 Rename.succVar (s1.val v) where
+  var := fun x => by simp [Store.lookup, Rename.succVar]
