Semantic/Stlc/Debruijn.lean
@@ -1,3 +1,4 @@
+import Mathlib.Tactic
 /-!
 Library for De Bruijn indices and parallel operations.
 -/
@@ -22,3 +23,14 @@ def Rename.succVar : Rename n (n+1) where
 
 def Rename.comp (f1 : Rename n1 n2) (f2 : Rename n2 n3) : Rename n1 n3 where
   var := fun x => f2.var (f1.var x)
+
+theorem Rename.funext {f1 f2 : Rename n1 n2}
+  (hvar : ∀ x, f1.var x = f2.var x) :
+  f1 = f2 := by
+  cases f1; cases f2
+  aesop
+
+theorem Rename.succVar_comm {f : Rename n1 n2} :
+  f.comp Rename.succVar = Rename.succVar.comp (f.liftVar) := by
+  apply Rename.funext
+  intro x; rfl
