Semantic/Stlc/Denotation.lean
@@ -1,0 +1,35 @@
+import Semantic.Stlc.TypeSystem
+import Semantic.Stlc.Interpreter
+import Mathlib.Tactic
+
+mutual
+
+def Ty.val_denot : Ty -> ∀ {n}, Config n -> Prop
+| .bool => fun config =>
+  config.e.is_bool_val
+| .nat => fun config =>
+  config.e.is_num_val
+| .arrow T U => fun config =>
+  ∀ arg_v,
+    Ty.val_denot T ⟨config.s, arg_v⟩ ->
+    Ty.exp_denot U ⟨config.s, .app config.e arg_v⟩
+
+def Ty.exp_denot : Ty -> ∀ {n}, Config n -> Prop
+| T => fun config =>
+  ∃ v,
+    Eval config.s config.e v
+    ∧ Ty.val_denot T ⟨config.s, v⟩
+
+end
+
+def TypedStore : Store n -> Ctx n -> Prop
+| .empty, .empty => True
+| .val s v, .var Γ T =>
+  TypedStore s Γ ∧ Ty.val_denot T ⟨s, v⟩
+
+def SemanticTyping (Γ : Ctx n) (e : Exp n) (T : Ty) : Prop :=
+  ∀ s,
+    TypedStore s Γ ->
+    Ty.exp_denot T ⟨s, e⟩
+
+notation:65 Γ " ⊨ " e " : " T => SemanticTyping Γ e T
